src/examples/Kuiper.Mul.fst
@@ -1,7 +1,9 @@
 module Kuiper.Mul
+#lang-pulse
 
 open Kuiper
 module U64 = FStar.UInt64
+module SZ = FStar.SizeT
 
 unfold let op_String_Access = Seq.index
 
@@ -9,30 +11,31 @@ let smul (s1 : seq u64) (s2 : seq u64 { len s2 == len s1 })
   : GTot (sr : seq u64 { len sr == len s1 })
   = Seq.init (len s1) (fun i -> U64.mul_mod s1.[i] s2.[i])
 
-#lang-pulse
-
 [@@CPrologue "__global__"] // no KrmlPrivate, example
-fn kernel (#size : erased nat)
+fn kernel (#size : erased nat{size > 0}) (* do NOT use erased pos, inference suffers *)
   (a1 a2 ar : gpu_array u64 size)
   (s1 s2 : erased (seq u64))
-  (etid : erased tid_t)
-  (#_ : squash (len s1 == size /\ len s2 == size /\ gdim_x etid * bdim_x etid == size))
+  (#_ : squash (len s1 == size /\ len s2 == size))
+  (ebid : enatlt size)
   preserves
-    gpu ** thread_id etid **
+    gpu ** block_id size ebid **
     pts_to a1 #(1.0R /. size) s1 **
-    pts_to a2 #(1.0R /. size) s2
+    pts_to a2 #(1.0R /. size) s2 **
+    emp
   requires
-    gpu_pts_to_slice ar (thread_index etid) (thread_index etid + 1) 's
+    gpu_pts_to_slice ar ebid (ebid + 1) 's
   ensures
-    gpu_pts_to_slice ar (thread_index etid) (thread_index etid + 1) seq![(smul s1 s2).[thread_index etid]]
+    gpu_pts_to_slice ar ebid (ebid + 1) seq![(smul s1 s2).[ebid]]
 {
-  let tid = thread_idx_all ();
-  rewrite each thread_index etid as tid;
-  let v1 = gpu_array_read #_ #_ #0 #size a1 tid;
-  let v2 = gpu_array_read #_ #_ #0 #size a2 tid;
+  let bid = get_bid ();
+  rewrite each ebid as SZ.v bid;
+  assert (pure (bid >= 0));
+  assert (pure (bid < size));
+  let v1 = gpu_array_read #_ #_ #0 #size a1 bid;
+  let v2 = gpu_array_read #_ #_ #0 #size a2 bid;
   let v = FStar.UInt64.(v1 *%^ v2);
-  gpu_array_write #_ #_ #tid #(tid + 1) ar tid v;
-  (**)with sr. assert gpu_pts_to_slice ar tid (tid + 1) sr;
-  (**)Seq.lemma_eq_intro sr seq![(smul s1 s2).[thread_index etid]];
+  gpu_array_write #_ #_ #bid #(bid + 1) ar bid v;
+  (**)with sr. assert gpu_pts_to_slice ar bid (bid + 1) sr;
+  (**)Seq.lemma_eq_intro sr seq![(smul s1 s2).[ebid]];
   ()
 }
